Logic/Modal/Normal/Geach.lean
@@ -2,6 +2,7 @@ import Logic.Vorspiel.BinaryRelations
 import Logic.Modal.Normal.Formula
 import Logic.Modal.Normal.Axioms
 import Logic.Modal.Normal.Semantics
+import Logic.Modal.Normal.Soundness
 import Logic.Modal.Normal.Completeness
 
 /-!
@@ -127,9 +128,12 @@ instance : IsGeachLogic (𝐊𝟒 : AxiomSet β) where
   char := by aesop;
 
 @[simp]
-instance : IsGeachLogic (𝐒𝟒 : AxiomSet β) where
+instance : IsGeachLogic (LogicKT4 : AxiomSet β) where
   taples := [(0, 0, 1, 0), (0, 2, 1, 0)];
   char := by simp [LogicKT4]; aesop;
+
+@[simp]
+instance : IsGeachLogic (𝐒𝟒 : AxiomSet β) := inferInstance
 
 @[simp]
 instance : IsGeachLogic (𝐒𝟒.𝟐 : AxiomSet β) where
@@ -137,9 +141,12 @@ instance : IsGeachLogic (𝐒𝟒.𝟐 : AxiomSet β) where
   char := by simp [LogicS4Dot2]; sorry; -- aesop;
 
 @[simp]
-instance : IsGeachLogic (𝐒𝟓 : AxiomSet β) where
+instance : IsGeachLogic (LogicKT5 : AxiomSet β) where
   taples := [(0, 0, 1, 0), (1, 1, 0, 1)];
   char := by simp [LogicKT5]; aesop;
+
+@[simp]
+instance : IsGeachLogic (𝐒𝟓 : AxiomSet β) := inferInstance
 
 @[simp]
 instance : IsGeachLogic (𝐊𝐓𝟒𝐁 : AxiomSet β) where
@@ -149,84 +156,66 @@ instance : IsGeachLogic (𝐊𝐓𝟒𝐁 : AxiomSet β) where
 end Axioms
 
 @[simp]
-def GeachConfluencyAux (l : GeachTaple) (F : Frame α) := ∀ {x y z}, (F[l.i] x y) ∧ (F[l.j] x z) → ∃ u, (F[l.m] y u) ∧ (F[l.n] z u)
+def GeachConfluency (l : GeachTaple) (F : Frame α) := ∀ {x y z}, (F[l.i] x y) ∧ (F[l.j] x z) → ∃ u, (F[l.m] y u) ∧ (F[l.n] z u)
 
 @[simp]
-def GeachConfluency (l : List (GeachTaple)) (rel : α → α → Prop) : Prop :=
+def GeachConfluency.list (l : List (GeachTaple)) (rel : α → α → Prop) : Prop :=
   match l with
   | [] => True
-  | x :: xs => (GeachConfluencyAux x rel) ∧ (GeachConfluency xs rel)
+  | x :: xs => (GeachConfluency x rel) ∧ (GeachConfluency.list xs rel)
 
-class IsGeachConfluency (P : (α → α → Prop) → Prop) where
-  taples : List (GeachTaple)
-  char : ∀ (rel : α → α → Prop), P rel ↔ GeachConfluency taples rel
+namespace GeachConfluency
 
-section GeachConfluency
+lemma list_single_iff : (GeachConfluency.list [l] F) ↔ GeachConfluency l F := by simp;
 
-@[simp]
-instance : IsGeachConfluency (@Serial α) where
-  taples := [(0, 0, 1, 1)];
-  char := by simp [Symmetric]; aesop
+lemma serial_def : Serial F ↔ (GeachConfluency (0, 0, 1, 1) F) := by
+  simp [Symmetric];
+  aesop;
 
-@[simp]
-instance : IsGeachConfluency (@Reflexive α) where
-  taples := [(0, 0, 1, 0)];
-  char := by simp [Reflexive];
+lemma reflexive_def : Reflexive F ↔ (GeachConfluency (0, 0, 1, 0) F) := by
+  simp [Reflexive];
 
-@[simp]
-instance : IsGeachConfluency (@Symmetric α) where
-  taples := [(0, 1, 0, 1)];
-  char := by simp [Symmetric]; aesop;
+lemma symmetric_def : Symmetric F ↔ (GeachConfluency (0, 1, 0, 1) F) := by
+  simp [Symmetric];
+  aesop;
 
-@[simp]
-instance : IsGeachConfluency (@Transitive α) where
-  taples := [(0, 2, 1, 0)];
-  char := by simp [Transitive]; aesop
+lemma transitive_def : Transitive F ↔ (GeachConfluency (0, 2, 1, 0) F) := by
+  simp [Transitive];
+  aesop;
 
-@[simp]
-instance : IsGeachConfluency (@Euclidean α) where
-  taples := [(1, 1, 0, 1)];
-  char := by simp [Euclidean]; aesop
+lemma euclidean_def : Euclidean F ↔ (GeachConfluency (1, 1, 0, 1) F) := by
+  simp [Euclidean];
+  aesop;
 
-@[simp]
-instance : IsGeachConfluency (@Confluent α) where
-  taples := [(1, 1, 1, 1)]
-  char := by simp [Confluent];
+lemma confluent_def : Confluent F ↔ (GeachConfluency (1, 1, 1, 1) F) := by
+  simp [Confluent];
 
-@[simp]
-instance : IsGeachConfluency (@Extensive α) where
-  taples := [(0, 1, 0, 0)];
-  char := by
-    intros;
-    simp [Extensive];
-    constructor;
-    . intro h x y z hxy hxz;
-      have := h hxz;
-      subst hxy this;
-      trivial;
-    . intro h x y hyz;
-      have := h rfl hyz;
-      subst this;
-      trivial;
+lemma extensive_def : Extensive F ↔ (GeachConfluency (0, 1, 0, 0) F) := by
+  intros;
+  simp [Extensive];
+  constructor;
+  . intro h x y z hxy hxz;
+    have := h hxz;
+    subst hxy this;
+    trivial;
+  . intro h x y hyz;
+    have := h rfl hyz;
+    subst this;
+    trivial;
 
-@[simp]
-instance : IsGeachConfluency (@Functional α) where
-  taples := [(1, 1, 0, 0)];
-  char := by simp [Functional]; aesop
+lemma functional_def : Functional F ↔ (GeachConfluency (1, 1, 0, 0) F) := by
+  simp [Functional];
+  aesop
 
-@[simp]
-instance : IsGeachConfluency (@Dense α) where
-  taples := [(0, 1, 2, 0)];
-  char := by simp [Dense]; aesop
-
-lemma subset_GeachConfluency (h : l₁ ⊆ l₂) : (GeachConfluency l₂ F) → (GeachConfluency l₁ F) := by
-  induction l₁ with
-  | nil => simp;
-  | cons x xs ih => sorry;
+lemma dense_def : Dense F  ↔ (GeachConfluency (0, 1, 2, 0) F) := by
+  simp [Dense];
+  aesop;
 
 end GeachConfluency
 
-theorem AxiomGeach.defines (F : Frame α) : (GeachConfluencyAux l F) ↔ (⊧ᴹ[F] (AxiomGeach.set l : AxiomSet β)) := by
+section FrameClassDefinability
+
+theorem AxiomGeach.defines (t : GeachTaple) (F : Frame α) : (GeachConfluency t F) ↔ (⊧ᴹ[F] (AxiomGeach.set t : AxiomSet β)) := by
   simp [AxiomGeach.set];
   constructor;
   . intro h p V x;
@@ -244,67 +233,51 @@ theorem AxiomGeach.defines (F : Frame α) : (GeachConfluencyAux l F) ↔ (⊧ᴹ
   . intro h x y z hi hj;
     let M : Model α β := {
       frame := F,
-      val := λ v _ => F[l.m] y v
+      val := λ v _ => F[t.m] y v
     }
-    have him : x ⊩ᴹ[M] ◇[l.i](□[l.m](Formula.atom default)) := by aesop;
+    have him : x ⊩ᴹ[M] ◇[t.i](□[t.m](Formula.atom default)) := by aesop;
     have := h (Formula.atom default) M.val x |>.modus_ponens him;
     simp only [Formula.Satisfies.multibox_def] at this;
     obtain ⟨u, hzu, hyu⟩ := by simpa using this z hj;
     existsi u;
     exact ⟨hyu, hzu⟩;
 
-lemma AxiomGeach.FrameClassDefinability : @FrameClassDefinability α β (AxiomGeach.set t) (GeachConfluencyAux t) := by
+lemma AxiomGeach.FrameClassDefinability (t : GeachTaple) : FrameClassDefinability α β (AxiomGeach.set t) (GeachConfluency t) := by
   intro F;
   have := @AxiomGeach.defines α β _ t F;
   constructor;
   . intro h p hp; exact this.mp h p hp;
   . aesop;
 
-lemma GeachLogic.FrameClassDefinability {l : List (GeachTaple)} : @FrameClassDefinability α β (GeachLogic l) (GeachConfluency l) := by
-  induction l with
+lemma GeachLogic.FrameClassDefinabilityAux {ts : List (GeachTaple)} : FrameClassDefinability α β (GeachLogic ts) (GeachConfluency.list ts) := by
+  induction ts with
   | nil => apply LogicK.FrameClassDefinability;
-  | cons head tail ih =>
+  | cons t ts ih =>
     simp only [GeachLogic, GeachConfluency, Normal.FrameClassDefinability, AxiomSetFrameClass.union];
     intro F;
     constructor;
     . intro h;
-      exact Set.mem_inter (ih.mp h.2) (AxiomGeach.FrameClassDefinability.mp h.1)
+      exact Set.mem_inter (ih.mp h.2) (AxiomGeach.FrameClassDefinability t |>.mp h.1)
     . intro h;
-      exact ⟨AxiomGeach.FrameClassDefinability.mpr h.2, ih.mpr h.1⟩;
+      exact ⟨AxiomGeach.FrameClassDefinability t |>.mpr h.2, ih.mpr h.1⟩;
 
-lemma AxiomSetFrameClass.geach
-  {Λ : AxiomSet β}
-  [hG : IsGeachLogic Λ]
-  : (𝔽(Λ) : FrameClass α) = (𝔽((GeachLogic hG.taples : AxiomSet β))) := by
-  exact Set.eq_of_subset_of_subset
-    (by
-      intro F hF;
-      apply GeachLogic.FrameClassDefinability |>.mp;
-      sorry;
-    )
-    (by
-      intro F hF;
-      have := GeachLogic.FrameClassDefinability |>.mpr hF;
-      sorry;
-    );
+lemma GeachLogic.FrameClassDefinability [hG : IsGeachLogic Λ] : FrameClassDefinability α β Λ (GeachConfluency.list hG.taples) := by
+  have := @GeachLogic.FrameClassDefinabilityAux α β _ hG.taples;
+  rw [←hG.char] at this;
+  simpa;
 
-lemma AxiomSetFrameClass.geach_subset (h : l₁ ⊆ l₂) : (𝔽((GeachLogic l₂ : AxiomSet β)) : FrameClass α) ⊆ 𝔽((GeachLogic l₁ : AxiomSet β)) := by
-  intro F hF;
-  have := GeachLogic.FrameClassDefinability |>.mpr hF;
-  apply GeachLogic.FrameClassDefinability |>.mp;
-  exact subset_GeachConfluency h this;
+lemma LogicS4.FrameClassDefinability : FrameClassDefinability α β 𝐒𝟒 (λ F => Reflexive F ∧ Transitive F) := by
+  have : Normal.FrameClassDefinability α β 𝐒𝟒 (GeachConfluency.list (IsGeachLogic.taples 𝐒𝟒)) := by apply GeachLogic.FrameClassDefinability;
+  simp_all [GeachConfluency.reflexive_def, GeachConfluency.transitive_def];
 
-lemma AxiomSetFrameClass.geach_subset' (h : l₁ ⊆ l₂) : (𝔽(𝐊 ∪ (GeachLogic l₂ : AxiomSet β)) : FrameClass α) ⊆ 𝔽(𝐊 ∪ (GeachLogic l₁ : AxiomSet β)) := by
-  repeat rw [AxiomSetFrameClass.union];
-  gcongr;
-  apply geach_subset h;
+end FrameClassDefinability
 
 namespace CanonicalModel
 
 variable [DecidableEq β]
 variable {Λ : AxiomSet β} (hK : 𝐊 ⊆ Λ)
 
-lemma defAxiomGeach (hG : (AxiomGeach.set l) ⊆ Λ) : (GeachConfluencyAux l) (CanonicalModel Λ).frame := by
+lemma defAxiomGeach (hG : (AxiomGeach.set l) ⊆ Λ) : (GeachConfluency l) (CanonicalModel Λ).frame := by
   intro Ω₁ Ω₂ Ω₃ h;
   replace ⟨h₁₂, h₂₃⟩ := h;
   replace h₁₂ : ∀ {p : Formula β}, p ∈ Ω₂ → ◇[GeachTaple.i l]p ∈ Ω₁ := multiframe_dia.mp h₁₂;
@@ -323,11 +296,11 @@ lemma defAxiomGeach (hG : (AxiomGeach.set l) ⊆ Λ) : (GeachConfluencyAux l) (C
     right;
     sorry;
 
-lemma defLogicGeach {l : List (GeachTaple)} (hG : (GeachLogic l) ⊆ Λ) : (GeachConfluency l) (CanonicalModel Λ).frame := by
+lemma defLogicGeach {l : List (GeachTaple)} (hG : (GeachLogic l) ⊆ Λ) : (GeachConfluency.list l) (CanonicalModel Λ).frame := by
   induction l with
   | nil => simp;
   | cons head tail ih =>
-    simp only [GeachLogic, GeachConfluency];
+    simp only [GeachLogic, GeachConfluency.list];
     constructor;
     . apply CanonicalModel.defAxiomGeach; aesop;
     . exact ih (by aesop);
@@ -339,7 +312,7 @@ variable [DecidableEq β]
 def GeachLogic.CanonicalModel (l : List (GeachTaple)) := Normal.CanonicalModel (GeachLogic l : AxiomSet β)
 
 lemma GeachLogic.membership_frameclass : (CanonicalModel l).frame ∈ (𝔽((GeachLogic l : AxiomSet β)) : FrameClass (MaximalConsistentTheory (GeachLogic l : AxiomSet β))) := by
-  apply FrameClassDefinability.mp;
+  apply FrameClassDefinabilityAux |>.mp;
   cases l with
   | nil => simp;
   | cons head tail =>
@@ -348,7 +321,7 @@ lemma GeachLogic.membership_frameclass : (CanonicalModel l).frame ∈ (𝔽((Gea
     . exact CanonicalModel.defAxiomGeach (by simp);
     . exact CanonicalModel.defLogicGeach (by simp);
 
-theorem GeachLogic.kripkeCompletesAux (l : List (GeachTaple)) : Completeness (GeachLogic l : AxiomSet β) (𝔽((GeachLogic l : AxiomSet β)) : FrameClass (MaximalConsistentTheory (GeachLogic l : AxiomSet β))) := by
+theorem GeachLogic.kripkeCompletesAux (l : List (GeachTaple)) : KripkeCompleteness (GeachLogic l : AxiomSet β) (𝔽((GeachLogic l : AxiomSet β)) : FrameClass (MaximalConsistentTheory (GeachLogic l : AxiomSet β))) := by
   apply completeness_def.mpr;
   intro Γ hConsisΓ;
   let ⟨Ω, hΩ⟩ := exists_maximal_consistent_theory hConsisΓ;
@@ -359,18 +332,18 @@ theorem GeachLogic.kripkeCompletesAux (l : List (GeachTaple)) : Completeness (Ge
     apply truthlemma' (by simp) |>.mpr;
     assumption;
 
-lemma GeachLogic.kripkeCompletes {Λ : AxiomSet β} [hG : IsGeachLogic Λ] : Completeness Λ (𝔽(Λ) : FrameClass (MaximalConsistentTheory Λ)) := by
+lemma GeachLogic.kripkeCompletes {Λ : AxiomSet β} [hG : IsGeachLogic Λ] : KripkeCompleteness Λ (𝔽(Λ) : FrameClass (MaximalConsistentTheory Λ)) := by
   rw [hG.char];
   apply GeachLogic.kripkeCompletesAux hG.taples;
 
-theorem LogicK.kripkeCompletes : Completeness (LogicK : AxiomSet β) (𝔽((LogicK : AxiomSet β)) : FrameClass (MaximalConsistentTheory (LogicK : AxiomSet β))) := GeachLogic.kripkeCompletes
+theorem LogicK.kripkeCompletes : KripkeCompleteness (LogicK : AxiomSet β) (𝔽((LogicK : AxiomSet β)) : FrameClass (MaximalConsistentTheory (LogicK : AxiomSet β))) := GeachLogic.kripkeCompletes
 
-theorem LogicKD.kripkeCompletes : Completeness (LogicKD : AxiomSet β) (𝔽((LogicKD : AxiomSet β)) : FrameClass (MaximalConsistentTheory (LogicKD : AxiomSet β))) := GeachLogic.kripkeCompletes
+theorem LogicKD.kripkeCompletes : KripkeCompleteness (LogicKD : AxiomSet β) (𝔽((LogicKD : AxiomSet β)) : FrameClass (MaximalConsistentTheory (LogicKD : AxiomSet β))) := GeachLogic.kripkeCompletes
 
-theorem LogicS5.kripkeCompletes : Completeness (LogicS5 : AxiomSet β) (𝔽((LogicS5 : AxiomSet β)) : FrameClass (MaximalConsistentTheory (LogicS5 : AxiomSet β))) := GeachLogic.kripkeCompletes
+theorem LogicS5.kripkeCompletes : KripkeCompleteness (LogicS5 : AxiomSet β) (𝔽((LogicS5 : AxiomSet β)) : FrameClass (MaximalConsistentTheory (LogicS5 : AxiomSet β))) := GeachLogic.kripkeCompletes
 
-theorem LogicS4.kripkeCompletes : Completeness (LogicS4 : AxiomSet β) (𝔽((LogicS4 : AxiomSet β)) : FrameClass (MaximalConsistentTheory (LogicS4 : AxiomSet β))) := GeachLogic.kripkeCompletes
+theorem LogicS4.kripkeCompletes : KripkeCompleteness (LogicS4 : AxiomSet β) (𝔽((LogicS4 : AxiomSet β)) : FrameClass (MaximalConsistentTheory (LogicS4 : AxiomSet β))) := GeachLogic.kripkeCompletes
 
-theorem LogicS4Dot2.kripkeCompletes : Completeness (LogicS4Dot2 : AxiomSet β) (𝔽((LogicS4Dot2 : AxiomSet β)) : FrameClass (MaximalConsistentTheory (LogicS4Dot2 : AxiomSet β))) := GeachLogic.kripkeCompletes
+theorem LogicS4Dot2.kripkeCompletes : KripkeCompleteness (LogicS4Dot2 : AxiomSet β) (𝔽((LogicS4Dot2 : AxiomSet β)) : FrameClass (MaximalConsistentTheory (LogicS4Dot2 : AxiomSet β))) := GeachLogic.kripkeCompletes
 
 end LO.Modal.Normal
